src/basic/FStarC.Errors.Codes.fst
@@ -394,5 +394,6 @@ let default_settings : list error_setting =
     Warning_CustardGeneratedNameInInterface            , CWarning, 377;
     Error_CustardBadLift                               , CAlwaysError, 378;
     Error_CustardDanglingReference                     , CAlwaysError, 379;
+    Error_CustardBadFloatLiteral                       , CAlwaysError, 380;
     Error_AmbiguousName                               , CError, 362;
     ]
