src/basic/FStarC.Errors.Codes.fsti
@@ -404,6 +404,7 @@ type error_code =
   | Warning_CustardGeneratedNameInInterface
   | Error_CustardBadLift
   | Error_CustardDanglingReference
+  | Error_CustardBadFloatLiteral
   | Error_AmbiguousName
 
 type error_setting = error_code & error_flag & int
